src/learnitreespaper.v
@@ -1,0 +1,231 @@
+From Coq Require Import
+Lists.List
+Strings.String
+Morphisms
+ZArith
+Setoid
+RelationClasses.
+
+(*Turning off some of the notation 
+helps to see what rules might be helpful*)
+
+From ITree Require Import
+    Eq.Eqit
+    Basics.Category
+    Basics.HeterogeneousRelations
+    Basics.Monad
+    Basics.CategorySub
+    Basics.CategoryOps
+    Interp.InterpFacts
+    Events.MapDefault
+    Events.MapDefaultFacts
+    Events.State
+    Events.StateFacts
+    ITreeMonad
+    ITreeFacts
+    ITree.
+
+From ExtLib Require Import
+    Core.RelDec
+    Structures.Monad
+    Structures.Maps
+    Programming.Show
+    Data.Map.FMapAList.
+
+Import CatNotations.
+Local Open Scope cat_scope.
+Local Open Scope itree_scope.
+
+From ITreeTutorial Require Import 
+    Fin 
+    Asm 
+    AsmCombinators 
+    AsmOptimization
+    Imp2Asm
+    KTreeFin
+    Utils_tutorial.
+
+Import ITreeNotations.
+
+Import ListNotations.
+Open Scope string_scope.
+
+Import CatNotations.
+Local Open Scope cat_scope.
+Local Open Scope itree_scope.
+
+From ITreeTutorial Require Import Fin Asm AsmCombinators Utils_tutorial.
+
+(* This serves as a general cheat sheet for the equational theory to reason 
+    about Itrees, general interpreters, specific interpreters, 
+    ktrees, *)
+
+Module section2.
+(* 2.1*)
+
+(* Monad Laws 
+
+    These exist in theories/Basic/Monad
+                   theories/Eq/Eqit
+*)
+
+Check bind_ret_l.
+Check bind_ret_r.
+Check bind_bind.
+
+(* Structural Laws *)
+Check bind_tau.
+Check bind_vis.
+Check bind_trigger.
+Check unfold_iter.
+
+(* Congruences 
+theories/Eq/Eqit
+
+https://github.com/DeepSpec/InteractionTrees/blob/dda104937d79e2052d1a26f6cbe89429245ff743/theories/Eq/Eqit.v#L1060
+*)
+Check eqit_Tau.
+Check eqit_Vis.
+Check eqit_Ret.
+Check eqit_bind_clo.
+Check eutt_clo_bind.
+Check eutt_Tau.
+
+
+
+(* 2.2 *)
+
+(* figure 6, ktree operations
+https://github.com/DeepSpec/InteractionTrees/blob/dda104937d79e2052d1a26f6cbe89429245ff743/theories/Basics/CategoryOps.v#L3C1-L3C1
+*)
+Check eq2.
+Check id_.
+Check cat.
+Check empty.
+Check one.
+Check bimap.
+Check case_.
+Check inl_.
+Check inr_.
+
+
+(* figure 7 laws for ktrees and handlers
+https://github.com/DeepSpec/InteractionTrees/blob/dda104937d79e2052d1a26f6cbe89429245ff743/theories/Basics/CategoryKleisliFacts.v
+*)
+Check compose_pure.
+Check assoc_r.
+Check unit_l.
+Check pure_cat.
+Check cat_pure.
+Check pure_inl.
+Check pure_inr.
+Check case_pure.
+Check case_l.
+Check bimap_id_pure.
+
+
+End section2.
+
+Module section3.
+
+(* 3.1
+ interpreting state events
+*)
+Check interp_state_ret.
+Check interp_state_vis.
+Check interp_state_tau.
+Check interp_state_trigger_eqit.
+Check interp_state_bind.
+Check interp_state_trigger.
+Check eutt_eq_interp_state_iter.
+Check eutt_interp_state_loop.
+(* https://github.com/DeepSpec/InteractionTrees/blob/dda104937d79e2052d1a26f6cbe89429245ff743/theories/Events/StateFacts.v#L120
+*)
+
+(* 3.2 
+monadic interpeters
+https://github.com/DeepSpec/InteractionTrees/blob/dda104937d79e2052d1a26f6cbe89429245ff743/theories/Interp/InterpFacts.v#L88
+*)
+Check interp_ret.
+Check interp_tau.
+Check interp_vis.
+Check interp_trigger.
+Check interp_bind.
+Check interp_interp.
+Check interp_iter.
+Check interp_loop.
+
+End section3.
+
+
+Module section4.
+
+(* iteration and recursion laws 
+https://github.com/DeepSpec/InteractionTrees/blob/dda104937d79e2052d1a26f6cbe89429245ff743/theories/Basics/CategoryFacts.v#L753C7-L753C25
+theories/basic/categoryfacts
+*)
+Check iter. 
+Check loop. 
+Check loop_natural_left.
+Check loop_vanishing_1.
+Check loop_dinatural.
+End section4.
+
+
+Module tactics.
+
+Print cat_auto.
+End tactic.
+
+
+
+(* learn loop construct*)
+Module loops.
+
+Print loop.
+(* loop := inr_ >>> iter (f >>> bimap inl_ (id_ b))
+
+so what are the sub components?
+*)
+
+Inductive void : Type -> Type :=.
+
+Definition M := itree void.
+
+Definition k1 : ktree void unit nat 
+    := fun tt => Ret 7.
+Definition k2 : ktree void nat nat
+    := fun n => Ret (n + 1).
+Definition k3 : ktree void unit bool 
+    := fun tt => Ret true.
+
+Definition k4 : ktree void (unit + nat) nat
+    := case_ k1 k2.
+    
+Eval compute in (inl_ >>> k4).
+
+Definition k5 : ktree void unit nat
+    := inl_ >>> k4.
+
+Definition k6 : ktree void unit nat
+    := pure (fun tt => 7).
+
+Definition k7 : ktree void (unit + unit) (nat + bool) 
+    := bimap k1 k3.
+
+
+Print bimap.
+Check k5.
+
+
+
+Definition ex1 : ktree void unit nat := 
+    k1 >>> k2.
+
+
+Definition ex1 (t : M nat) : M (unit * nat) := inr_ unit t.
+
+Print inr_.
+Print Inr.
+
+End loops.
